src/eqdec.ml4
@@ -38,7 +38,7 @@ open Typeops
 open Type_errors
 open Pp
 open Proof_type
-
+open Errors
 open Glob_term
 open Retyping
 open Pretype_errors
